wip

src/Init/Control/MonadAttach.lean
@@ -16,3 +16,12 @@ public class LawfulMonadAttach (m : Type u → Type v) [Monad m] [MonadAttach m]
   map_attach {α : Type u} {x : m α} : Subtype.val <$> MonadAttach.attach x = x
   canReturn_map_imp {α : Type u} {P : α → Prop} {x : m (Subtype P)} {a : α} :
       MonadAttach.CanReturn (Subtype.val <$> x) a → P a
+  map_some_inj {α : Type u} {x y : m α} : some <$> x = some <$> y → x = y
+  -- attach_distrib {α β : Type u} {x : m α} {f : α → m β} :
+  --   (fun ⟨fa, hfa⟩ => ⟨fa, sorry⟩) <$> MonadAttach.attach (x >>= f) =
+  --     MonadAttach.attach x >>= (fun ⟨a, ha⟩ => (fun ⟨fa, hfa⟩ => Subtype.mk fa (Exists.intro a (And.intro ha hfa))) <$> MonadAttach.attach (f a))
+
+public def MonadAttach.pbind
+    [Monad m] [MonadAttach m]
+    (x : m α) (f : (a : α) → MonadAttach.CanReturn x a → m β) : m β :=
+  MonadAttach.attach x >>= (fun ⟨a, ha⟩ => f a ha)
